start proof of recv case for a timeout<->state query invariant

systems/chord-props/QueryInvariant.v
@@ -10,45 +10,6 @@ Require Import Chord.SystemReachable.
 
 Set Bullet Behavior "Strict Subproofs".
 
-Ltac start_cases :=
-  match goal with
-  | [H : ?h' = ?h \/ _,
-     H' : update _ (timeouts ?gst) ?h' _ ?h = _ ++ _ :: _
-     |- _] =>
-    destruct H
-  end.
-
-Ltac fail_cases :=
-  idtac.
-
-Ltac timeout_cases :=
-  idtac.
-
-Ltac recv_cases :=
-  idtac.
-
-Ltac input_cases :=
-  idtac.
-
-Ltac client_cases :=
-  idtac.
-
-Ltac step_dynamic_cases :=
-  match goal with
-  | H : step_dynamic ?gst ?gst' |- _ =>
-    invcs H;
-    [ start_cases
-    | fail_cases
-    | timeout_cases
-    | recv_cases
-    | input_cases
-    | client_cases
-    ];
-    subst_max;
-    rewrite_update;
-    try find_injection
-  end.
-
 Definition at_most_one_request_timeout (gst : global_state) (h : addr) :=
   forall xs ys dst p,
     timeouts gst h = xs ++ Request dst p :: ys ->
@@ -224,6 +185,85 @@ Proof.
     find_false;
     intuition.
 Qed.
+
+Hint Resolve live_node_characterization.
+
+Inductive cur_request_timeouts_related (gst : global_state) (h : addr) : Prop :=
+| QSTNoRequest :
+    forall st,
+      sigma gst h = Some st ->
+      (forall dst req, ~ In (Request dst req) (timeouts gst h)) ->
+      cur_request st = None ->
+      cur_request_timeouts_related gst h
+| QSTRequest :
+    forall st dstp q req,
+      sigma gst h = Some st ->
+      query_request q req ->
+      In (Request (addr_of dstp) req) (timeouts gst h) ->
+      cur_request st = Some (dstp, q, req) ->
+      cur_request_timeouts_related gst h.
+Hint Constructors cur_request_timeouts_related.
+
+Lemma cur_request_timeouts_related_equiv_st :
+  forall gst gst' h,
+    sigma gst h = sigma gst' h ->
+    timeouts gst h = timeouts gst' h ->
+    cur_request_timeouts_related gst h ->
+    cur_request_timeouts_related gst' h.
+Proof.
+  intros.
+  inv_prop cur_request_timeouts_related;
+    repeat find_rewrite; eauto.
+Qed.
+
+Definition live_node_cur_request_timeouts_related (gst : global_state) : Prop :=
+  forall h,
+    In h (nodes gst) ->
+    ~ In h (failed_nodes gst) ->
+    cur_request_timeouts_related gst h.
+Hint Unfold live_node_cur_request_timeouts_related.
+
+Lemma cur_request_timeouts_related_recv_invariant :
+  chord_recv_handler_invariant live_node_cur_request_timeouts_related.
+Proof.
+  autounfold; intros.
+  destruct (addr_eq_dec h0 h).
+  - subst; rewrite_update.
+    assert (cur_request_timeouts_related gst h)
+      by (repeat find_rewrite; auto).
+    find_copy_eapply_lem_hyp recv_handler_possible_nts.
+    find_copy_eapply_lem_hyp recv_handler_possible_cts.
+    inv_prop cur_request_timeouts_related.
+    + destruct nts.
+      * destruct (cur_request st') as [[[? ?] ?]|] eqn:?.
+        -- (* need lemma like handle_query_res_info_from_changed_set_cur_request
+              but for recv_handler *)
+          admit.
+        -- econstructor; eauto;
+             repeat find_rewrite; rewrite_update; simpl; auto.
+           autounfold; intros.
+           find_apply_lem_hyp in_remove_all_was_in.
+           cut (~ In (Request dst req) (timeouts gst h)); [intuition|].
+           inv_prop cur_request_timeouts_related; eauto.
+      * repeat (handler_def || handler_simpl ||
+                match goal with
+                | H : context[recv_handler] |- _ =>
+                  eapply recv_handler_sets_cur_request_when_adding_new_timeout in H; eauto with datatypes;
+                  expand_def;
+                  econstructor 2;
+                  repeat find_rewrite;
+                  try rewrite update_eq;
+                  eauto with datatypes
+                end).
+        econstructor; repeat find_rewrite; rewrite_update; eauto with datatypes.
+        autounfold; intros; simpl in *; break_or_hyp; try congruence.
+        cut (In (Request dst req) (timeouts gst h)); [eauto|].
+        eapply in_remove; eauto.
+    + admit.
+  - assert (cur_request_timeouts_related gst h0) by (repeat find_rewrite; auto).
+    find_eapply_lem_hyp cur_request_timeouts_related_equiv_st; eauto;
+      repeat find_rewrite; rewrite_update; reflexivity.
+Admitted.
 
 Lemma open_request_with_response_on_wire_closed_or_preserved :
   forall gst l gst' src dst req res,
